update to the prototype

sample.bpl
@@ -1,53 +1,180 @@
 // Program
-var $M: [Machine] Machine;
-
-//var $Heap: <T>[int, Field T] T;
-var $Heap: [int, int] int;
-//var $State: [int] State;
-var $State: [int] int;
+var $MType: [int] Machine;
 var $CurrMid: int;
 
-const unique $NULL: int;
-axiom $NULL == 0;
+var $Heap: [int, int] int;
+var $State: [int] State;
+var $Raised: [int] Event;
+
+var $Inbox: [int, int] Event;
+var $InboxSize: [int] int;
 
 
 // Types
-type Event;
 type Machine;
-//type State;
-//type Field _;
+type State;
 type Fun;
+type Event = int;
+
+const unique $HALT: Event;
+const unique $DEFAULT: Event;
+const unique $NULL: int;
+
 
 // Machinery
 procedure {:inline 1} $create_machine(m: Machine) returns (r: int);
-  modifies $CurrMid;
+  modifies $CurrMid, $MType, $InboxSize;
 
 implementation {:inline 1} $create_machine(m: Machine) returns (r: int)
 {
+  var mid: int;
+
   $bb0:
     assume $CurrMid > 0;
-    r := $CurrMid;
+    mid := $CurrMid;
     $CurrMid := $CurrMid + 1;
+
+    $InboxSize[mid] := 0;
 
     if (m == _machine.server)
     {
+      $MType[mid] := _machine.server;
       async call _machine.server.constructor(r);
     }
     else if (m == _machine.client)
     {
+      $MType[mid] := _machine.client;
       async call _machine.client.constructor(r);
     }
+
+    r := mid;
     return;
 }
 
-procedure {:inline 1} $raise(mid: int);
+procedure {:inline 1} $raise(mid: int, e: Event);
+  modifies $State, $Raised, $Inbox, $InboxSize;
 
-implementation {:inline 1} $raise(mid: int)
+implementation {:inline 1} $raise(mid: int, e: Event)
 {
   $bb0:
-    assert false;
+    $Raised[mid] := e;
+    call $handle_event(mid);
     return;
 }
+
+procedure {:inline 1} $send(mid: int, e: Event);
+  modifies $Inbox, $InboxSize;
+
+implementation {:inline 1} $send(mid: int, e: Event)
+{
+  $bb0:
+    call $enqueue(mid, e);
+    async call $handle_event(mid);
+    return;
+}
+
+procedure {:inline 1} $enqueue(mid: int, e: Event);
+  modifies $Inbox, $InboxSize;
+
+implementation {:inline 1} $enqueue(mid: int, e: Event)
+{
+  var index: int;
+
+  $bb0:
+    index := $InboxSize[mid];
+    $Inbox[mid, index] := e;
+    $InboxSize[mid] := $InboxSize[mid] + 1;
+    return;
+}
+
+procedure {:inline 1} $get_next_event(mid: int) returns (r: Event);
+  modifies $Raised;
+
+implementation {:inline 1} $get_next_event(mid: int) returns (r: Event)
+{
+  $bb0:
+    r := $NULL;
+
+    if ($Raised[mid] != $NULL)
+    {
+      r := $Raised[mid];
+      $Raised[mid] := $NULL;
+    }
+    else if ($InboxSize[mid] > 0)
+    {
+
+      // while (true)
+      // {
+      //   break;
+      //   // assert false;
+      // }
+      assert false;
+    }
+
+    return;
+}
+
+procedure {:inline 1} $handle_event(mid: int);
+  modifies $State, $Raised, $Inbox, $InboxSize;
+
+implementation {:inline 1} $handle_event(mid: int)
+{
+  var nextEvent: Event;
+
+  $bb0:
+    call nextEvent := $get_next_event(mid);
+
+    if ($MType[mid] == _machine.server)
+    {
+      if ($State[mid] == _machine.server.init)
+      {
+        if (nextEvent == _event.unit)
+        {
+          call $goto_state(mid, _machine.server.playing);
+        }
+      }
+      else if ($State[mid] == _machine.server.playing)
+      {
+        if (nextEvent == _event.unit)
+        {
+
+        }
+        else if (nextEvent == _event.ping)
+        {
+
+        }
+      }
+    }
+    else if ($MType[mid] == _machine.client)
+    {
+      if ($State[mid] == _machine.client.init)
+      {
+
+      }
+      else if ($State[mid] == _machine.client.playing)
+      {
+
+      }
+    }
+
+    return;
+}
+
+procedure {:inline 1} $goto_state(mid: int, s: State);
+  modifies $State, $Inbox, $InboxSize;
+
+implementation {:inline 1} $goto_state(mid: int, s: State)
+{
+  $bb0:
+    $State[mid] := s;
+    if (s == _machine.server.playing)
+    {
+      call _machine.server.playing.entry(mid);
+    }
+
+    return;
+}
+
 
 // Events
 const unique _event.ping: Event;
@@ -57,17 +184,16 @@ const unique _event.unit: Event;
 
 // Machine: server
 const {:main} unique _machine.server: Machine;
-const {:start} unique _machine.server.init: int;
-const unique _machine.server.playing: int;
+const {:start} unique _machine.server.init: State;
+const unique _machine.server.playing: State;
 
-//const unique _machine.server.client: Field int;
 const unique _machine.server.client: int;
 
 const {:entry} unique _machine.server.init.entry: Fun;
 const {:entry} unique _machine.server.playing.entry: Fun;
 
 procedure {:inline 1} _machine.server.constructor(mid: int);
-  modifies $CurrMid, $Heap, $State;
+  modifies $CurrMid, $MType, $Heap, $State, $Raised, $Inbox, $InboxSize;
 
 implementation {:inline 1} _machine.server.constructor(mid: int)
 {
@@ -75,58 +201,109 @@ implementation {:inline 1} _machine.server.constructor(mid: int)
     yield;
     $Heap[mid, _machine.server.client] := $NULL;
     $State[mid] := _machine.server.init;
+    $Raised[mid] := $NULL;
     call _machine.server.init.entry(mid);
     return;
 }
 
 procedure {:inline 1} _machine.server.init.entry(mid: int);
-  modifies $CurrMid, $Heap, $State;
+  modifies $CurrMid, $MType, $Heap, $State, $Raised, $Inbox, $InboxSize;
 
 implementation {:inline 1} _machine.server.init.entry(mid: int)
 {
   var client: int;
 
   $bb0:
-    call {:create} client := $create_machine(_machine.client);
+    call client := $create_machine(_machine.client);
     $Heap[mid, _machine.server.client] := client;
-    call {:raise} $raise(mid);
+    call $raise(mid, _event.unit);
+    return;
+}
+
+procedure {:inline 1} _machine.server.playing.entry(mid: int);
+  modifies $Inbox, $InboxSize;
+
+implementation {:inline 1} _machine.server.playing.entry(mid: int)
+{
+  $bb0:
+    call $send($Heap[mid, _machine.server.client], _event.pong);
+    return;
+}
+
+procedure {:inline 1} _machine.server.sendPong(mid: int);
+  modifies $Inbox, $InboxSize;
+
+implementation {:inline 1} _machine.server.sendPong(mid: int)
+{
+  $bb0:
+    call $send($Heap[mid, _machine.server.client], _event.pong);
     return;
 }
 
 
 // Machine: client
 const unique _machine.client: Machine;
-const {:start} unique _machine.client.init: int;
-const unique _machine.client.playing: int;
+const {:start} unique _machine.client.init: State;
+const unique _machine.client.playing: State;
 
-//const unique _machine.client.server: Field int;
 const unique _machine.client.server: int;
+const unique _machine.client.counter: int;
 
 const {:entry} unique _machine.client.init.entry: Fun;
 const {:entry} unique _machine.client.playing.entry: Fun;
 
 procedure {:inline 1} _machine.client.constructor(mid: int);
-  modifies $Heap, $State;
+  modifies $Heap, $State, $Raised;
 
 implementation {:inline 1} _machine.client.constructor(mid: int)
 {
   $bb0:
     yield;
     $Heap[mid, _machine.client.server] := $NULL;
+    $Heap[mid, _machine.client.counter] := 0;
     $State[mid] := _machine.client.init;
+    $Raised[mid] := $NULL;
+    return;
+}
+
+procedure {:inline 1} _machine.client.init.entry(mid: int);
+  modifies $CurrMid, $MType, $Heap, $State, $Raised;
+
+implementation {:inline 1} _machine.client.init.entry(mid: int)
+{
+  var client: int;
+
+  $bb0:
+    assert false;
+    return;
+}
+
+procedure {:inline 1} _machine.client.playing.entry(mid: int);
+
+implementation {:inline 1} _machine.client.playing.entry(mid: int)
+{
+  $bb0:
+    return;
+}
+
+procedure {:inline 1} _machine.client.sendPing(mid: int);
+
+implementation {:inline 1} _machine.client.sendPing(mid: int)
+{
+  $bb0:
     return;
 }
 
 
 // Entry point
 procedure {:entrypoint} Main();
-  modifies $CurrMid;
+  modifies $CurrMid, $MType, $InboxSize;
 
 implementation {:entrypoint} Main()
 {
   var m: int;
 
   $main:
-    call {:create} m := $create_machine(_machine.server);
+    call m := $create_machine(_machine.server);
     return;
 }
